Housekeeping

demo/fib/Fib2.v
@@ -6,6 +6,7 @@ Require Import SmallstepC.
 Require Export Simulation.
 Require Import Skeleton Mod ModSem.
 Require ClightC.
+Require Import FibHeader.
 Require Import Fib0.
 Require Import SIR.
 (* Require Import Clightdefs. *)
@@ -14,13 +15,10 @@ Set Implicit Arguments.
 
 
 
-Definition owned_heap: Type := unit.
-Definition initial_owned_heap: SkEnv.t -> owned_heap := fun _ => tt.
-
-Definition f_fib (oh0: owned_heap) (m0: mem) (vs: list val):
+Definition f_fib (oh0: owned_heap) (m0: mem) (vs0: list val):
   itree (E owned_heap) (owned_heap * (mem * val)) :=
   tau;;
-  match vs with
+  match vs0 with
   | [Vint n] =>
     if Int.eq n Int.zero
     then Ret (oh0, (m0, (Vint Int.zero)))
