demo/fib/Fib3.v
@@ -6,6 +6,7 @@ Require Import SmallstepC.
 Require Export Simulation.
 Require Import Skeleton Mod ModSem.
 Require ClightC.
+Require Import FibHeader.
 Require Import Fib0.
 Require Import SIR.
 (* Require Import Clightdefs. *)
@@ -13,81 +14,6 @@ Require Import SIR.
 Set Implicit Arguments.
 
 
-
-Definition owned_heap: Type := unit.
-Definition initial_owned_heap: SkEnv.t -> owned_heap := fun _ => tt.
-
-
-(* Definition to_nat (i: int): nat := Z.to_nat (Int.unsigned i). *)
-Definition to_nat (i: int): nat := Z.to_nat (Int.signed i).
-Definition of_nat (n: nat): int := Int.repr (Z.of_nat n).
-
-Definition to_nat_opt (i: int): option nat :=
-  if zle 0 (Int.signed i)
-  then Some (Z.to_nat (Int.signed i))
-  else None
-.
-
-Definition of_nat_opt (n: nat): option int :=
-  if zlt (Z.of_nat n) Int.modulus
-  then Some (Int.repr (Z.of_nat n))
-  else None
-.
-
-(* Goal forall x y (POS: Int.signed x + Int.signed y <= Int.max_signed) (POS: Int.signed x >= 0) (POS: Int.signed y >= 0), to_nat (Int.add x y) = Nat.add (to_nat x) (to_nat y). *)
-(* Proof. *)
-(*   i. unfold to_nat. *)
-(*   rewrite <- Z2Nat.inj_add; eauto with xomega. rewrite Int.add_signed. rewrite Int.signed_repr; ss. *)
-(*   split; try xomega. *)
-(*   - generalize Int.min_signed_neg; i. xomega. *)
-(* Qed. *)
-Fixpoint fib_nat (n: nat): nat :=
-  match n with
-  | 0%nat => 0%nat
-  | S n' =>
-    match n' with
-    | 0%nat => 1%nat
-    | S n'' => fib_nat n'' + fib_nat n'
-    end
-  end.
-
-(***
-precondition: exists n, vs = [Vint n]
-postcondition: OH unchanged && M unchanged && rv = of_nat (fib(n))
-***)
-
-(***
-Definition fib_spec fun_id :=
- DECLARE fun_id
-  WITH n : Z
-  PRE  [ _n OF tint ]
-     PROP (0 <= n < 45) (* 50th term is too large to be a 32bit int *)
-     LOCAL (temp _n (Vint (Int.repr n)))
-     SEP ()
-  POST [ tint ]
-     PROP () LOCAL (temp ret_temp (Vint (Int.repr (fib_of_Z n))))
-     SEP ().
-***)
-
-Definition parse_arg (oh0: owned_heap) (m0: mem) (vs0: list val): option nat :=
-  match vs0 with
-  | [Vint n] => (to_nat_opt n)
-  | _ => None
-  end
-.
-Hint Unfold parse_arg.
-
-Coercion is_some_coercion {X}: (option X) -> bool := is_some.
-Definition precond (oh0: owned_heap) (m0: mem) (vs0: list val) := exists n, parse_arg oh0 m0 vs0 = Some n.
-
-Definition postcond (oh0: owned_heap) (m0: mem) (vs0: list val): (owned_heap * (mem * val)) -> Prop :=
-  fun '(ohr, (mr, vr)) => 
-    match parse_arg oh0 m0 vs0 with
-    | Some n => (<<OH: oh0 = ohr>> /\ <<M: m0 = mr>> /\ <<V: vr = Vint (of_nat (fib_nat n))>>)
-    | _ => False
-    end
-.
-Hint Unfold postcond.
 
 Definition f_fib (oh0: owned_heap) (m0: mem) (vs0: list val):
   itree (E owned_heap) (owned_heap * (mem * val)) :=
@@ -116,33 +42,6 @@ Definition f_fib (oh0: owned_heap) (m0: mem) (vs0: list val):
 
   >>= guaranteeK (postcond oh0 m0 vs0)
 .
-(*     else *)
-(*       if Nat.eqb n 0%nat *)
-(* Definition f_fib (oh0: owned_heap) (m0: mem) (vs: list val): *)
-(*   itree (E owned_heap) (owned_heap * (mem * val)) := *)
-(*   tau;; *)
-(*   match vs with *)
-(*   | [Vint n] => *)
-(*     if Int.eq n Int.zero *)
-(*     then Ret (oh0, (m0, (Vint Int.zero))) *)
-(*     else *)
-(*       if Int.eq n Int.one *)
-(*       then Ret (oh0, (m0, (Vint Int.one))) *)
-(*       else *)
-(*         (* guarantee (Int_le n Int.zero) ;; *) *)
-(*         guarantee True ;; *)
-(*         '(oh1, (m1, y1)) <- trigger (ICall _fib oh0 m0 [Vint (Int.sub n (Int.repr 2))]) ;; *)
-(*         (assume (fun _ => <<OH: oh0 = oh1>> /\ <<M: m0 = m1 >> /\ <<V: y1 = fib (Int.sub n (Int.repr 2))>>) tt) ;; *)
-
-(*         guarantee True ;; *)
-(*         '(oh2, (m2, y2)) <- trigger (ICall _fib oh1 m1 [Vint (Int.sub n (Int.repr 1))]) ;; *)
-(*         assume (<<OH: oh1 = oh2>> /\ <<M: m1 = m2 >> /\ <<V: y2 = fib (Int.sub n (Int.repr 1))>>) ;; *)
-(*         Ret (oh2, (m2, Val.add y1 y2)) *)
-(*   | _ => triggerUB *)
-(*   end *)
-(*   >>= *)
-(*   (fun '(ohr, (mr, vr)) => guarantee(<<OH: oh0 = ohr>> /\ <<M: m0 = mr>> /\ <<V: True>>) ;; Ret (ohr, (mr, vr))) *)
-(* . *)
 
 Definition prog: program owned_heap := (Maps.add _fib f_fib Maps.empty).
 
