demo/fib/AuxBuffer.v
@@ -1,0 +1,98 @@
+Require Import CoqlibC Maps.
+Require Import ASTC IntegersC ValuesC EventsC MemoryC Globalenvs.
+Require Import Op Registers.
+Require Import sflib.
+Require Import SmallstepC.
+Require Export Simulation.
+Require Import Skeleton Mod ModSem.
+(* Require Import Clightdefs. *)
+
+Set Implicit Arguments.
+
+
+
+
+(*** nat ***)
+Lemma succ_pred
+      x y
+  :
+    <<SUCC: x = S y>> <-> <<PRED: (x - 1)%nat = y /\ (1 <= x)%nat>>
+.
+Proof.
+  {
+    split.
+    - ginduction x; ii; des; ss. clarify. split; try xomega.
+    - ginduction x; ii; des; clarify; ss; try xomega. f_equal. rewrite Nat.sub_0_r. ss.
+  }
+Qed.
+
+
+
+
+
+(*** int ***)
+Lemma eta
+      i j
+      (EQ: i.(Int.intval) = j.(Int.intval))
+  :
+    <<EQ: i = j>>
+.
+Proof.
+  r. destruct i, j; ss. clarify. f_equal. eapply Axioms.proof_irr.
+Qed.
+
+Lemma Int_add_repr: forall x y,
+    <<EQ: (Int.add (Int.repr x) (Int.repr y)) = Int.repr (x + y)>>.
+Proof.
+  i. apply Int.eqm_repr_eq. eapply Int.eqm_sym. eapply Int.eqm_trans.
+  - apply Int.eqm_sym. apply Int.eqm_unsigned_repr.
+  - apply Int.eqm_add; apply Int.eqm_unsigned_repr.
+Qed.
+
+Lemma Int_sub_repr: forall x y,
+    <<EQ: (Int.sub (Int.repr x) (Int.repr y)) = Int.repr (x - y)>>.
+Proof.
+  i. apply Int.eqm_repr_eq. eapply Int.eqm_sym. eapply Int.eqm_trans.
+  - apply Int.eqm_sym. apply Int.eqm_unsigned_repr.
+  - apply Int.eqm_sub; apply Int.eqm_unsigned_repr.
+Qed.
+
+
+
+
+
+
+
+(*** nat && int ***)
+Definition to_nat (i: int): nat := Z.to_nat (Int.signed i).
+Definition of_nat (n: nat): int := Int.repr (Z.of_nat n).
+
+Definition to_nat_opt (i: int): option nat :=
+  if zle 0 (Int.signed i)
+  then Some (Z.to_nat (Int.signed i))
+  else None
+.
+
+Definition of_nat_opt (n: nat): option int :=
+  if zlt (Z.of_nat n) Int.modulus
+  then Some (Int.repr (Z.of_nat n))
+  else None
+.
+Hint Unfold of_nat to_nat of_nat_opt to_nat_opt.
+
+Lemma range_to_nat
+      x
+      (RANGE: Z.of_nat x <= Int.max_signed)
+  :
+    to_nat_opt (of_nat x) = Some x
+.
+Proof.
+  { i. unfold to_nat_opt, of_nat.
+    generalize Int.min_signed_neg; i.
+    generalize (Int.signed_range (Int.repr (Z.of_nat x))); i.
+    rewrite Int.signed_repr in *; try lia. des_ifs; try lia.
+    rewrite Nat2Z.id; ss.
+  }
+Qed.
+
+
