demo/fib/FibHeader.v
@@ -1,0 +1,76 @@
+Require Import CoqlibC Maps.
+Require Import ASTC Integers ValuesC EventsC MemoryC Globalenvs.
+Require Import Op Registers.
+Require Import sflib.
+Require Import SmallstepC.
+Require Export Simulation.
+Require Import Skeleton Mod ModSem.
+Require ClightC.
+Require Import Fib0.
+Require Import SIR.
+Require Export AuxBuffer.
+(* Require Import Clightdefs. *)
+
+Set Implicit Arguments.
+
+
+
+Definition owned_heap: Type := unit.
+Definition initial_owned_heap: SkEnv.t -> owned_heap := fun _ => tt.
+
+Fixpoint fib_nat (n: nat): nat :=
+  match n with
+  | 0%nat => 0%nat
+  | S n' =>
+    match n' with
+    | 0%nat => 1%nat
+    | S n'' => fib_nat n'' + fib_nat n'
+    end
+  end.
+Lemma fib_nat_0: (fib_nat 0 = 0)%nat. Proof. ss. Qed.
+Lemma fib_nat_1: (fib_nat 1 = 1)%nat. Proof. ss. Qed.
+Lemma fib_nat_recurse: forall n, ((fib_nat (S (S n))) = (fib_nat n) + fib_nat (S n))%nat.
+Proof. reflexivity. Qed.
+Global Opaque fib_nat.
+
+(*** TODO: compare with VST (compile it!) ***)
+(***
+Definition fib_spec fun_id :=
+ DECLARE fun_id
+  WITH n : Z
+  PRE  [ _n OF tint ]
+     PROP (0 <= n < 45) (* 50th term is too large to be a 32bit int *)
+     LOCAL (temp _n (Vint (Int.repr n)))
+     SEP ()
+  POST [ tint ]
+     PROP () LOCAL (temp ret_temp (Vint (Int.repr (fib_of_Z n))))
+     SEP ().
+***)
+
+Definition parse_arg (oh0: owned_heap) (m0: mem) (vs0: list val): option nat :=
+  match vs0 with
+  | [Vint n] => (to_nat_opt n)
+  | _ => None
+  end
+.
+Hint Unfold parse_arg.
+
+(*** TODO: move to CoqlibC ***)
+Coercion is_some_coercion {X}: (option X) -> bool := is_some.
+Definition precond (oh0: owned_heap) (m0: mem) (vs0: list val) := exists n, parse_arg oh0 m0 vs0 = Some n.
+
+Definition postcond (oh0: owned_heap) (m0: mem) (vs0: list val): (owned_heap * (mem * val)) -> Prop :=
+  fun '(ohr, (mr, vr)) => 
+    match parse_arg oh0 m0 vs0 with
+    | Some n => (<<OH: oh0 = ohr>> /\ <<M: m0 = mr>> /\ <<V: vr = Vint (of_nat (fib_nat n))>>)
+    | _ => False
+    end
+.
+Hint Unfold postcond.
+
+(*** TODO: move to more root ***)
+Global Opaque ident_eq.
+Global Opaque Z.of_nat.
+
+
+Definition _fib_ru := 57%positive.
